SMS.v
@@ -6,30 +6,40 @@ From Elo Require Import Array.
 From Elo Require Import Map.
 From Elo Require Import Core.
 From Elo Require Import Contains.
+From Elo Require Import ValidAddresses.
 From Elo Require Import Access.
-From Elo Require Import ValidAccesses.
 From Elo Require Import References.
-From Elo Require Import AccessProp.
 From Elo Require Import UnsafeAccess.
 From Elo Require Import SafeSpawns.
 
-Local Definition safe_memory_sharing m ths := forall tid1 tid2 ad,
+Definition safe_memory_sharing m ths := forall tid1 tid2 ad,
   tid1 <> tid2 ->
   access m ths[tid2] ad ->
   ~ UnsafeAccess m ths[tid1] ad.
 
 (* ------------------------------------------------------------------------- *)
-(* mstep preservation                                                        *)
+(* helpers                                                                   *)
 (* ------------------------------------------------------------------------- *)
 
-Local Lemma length_tid : forall t ths tid eff,
+Local Lemma step_length_tid : forall t ths tid eff,
   ths[tid] --[eff]--> t ->
-  tid < length ths.
+  tid < #ths.
 Proof.
   intros * Hstep.
-  decompose sum (lt_eq_lt_dec tid (length ths)); subst; trivial;
+  decompose sum (lt_eq_lt_dec tid (#ths)); subst; trivial;
   simpl_array; try lia; inversion_step.
 Qed.
+
+Local Lemma cstep_length_tid : forall m m' ths ths' tid eff,
+  m / ths ~~[tid, eff]~~> m' / ths' ->
+  tid < #ths.
+Proof.
+  intros. inversion_clear_cstep; trivial.
+Qed.
+
+(* ------------------------------------------------------------------------- *)
+(* mstep preservation                                                        *)
+(* ------------------------------------------------------------------------- *)
 
 Local Lemma step_write_requires_uacc : forall m t t' ad v V T,
   empty |-- t is T ->
@@ -43,7 +53,7 @@ Qed.
 
 Local Lemma step_write_sms_helper : forall m t ad v ths tid tid' V,
   tid <> tid' ->
-  forall_threads ths well_typed_thread ->
+  forall_threads ths well_typed ->
   safe_memory_sharing m ths ->
   ths[tid] --[EF_Write ad v V]--> t ->
   ~ access m ths[tid'] ad.
@@ -59,7 +69,7 @@ Local Lemma step_none_sms_preservation : forall m t ths tid,
   safe_memory_sharing m ths[tid <- t].
 Proof.
   intros * ? ? tid1 tid2 ? ? ?.
-  assert (tid < length ths) by eauto using length_tid.
+  assert (tid < #ths) by eauto using step_length_tid.
   destruct (Nat.eq_dec tid tid1), (Nat.eq_dec tid tid2); subst; try lia;
   simpl_array;
   eauto using step_none_nuacc_preservation, step_none_inherits_access.
@@ -68,15 +78,15 @@ Qed.
 Local Lemma step_alloc_sms_preservation : forall m t v ths tid V,
   forall_threads ths (valid_accesses m) ->
   safe_memory_sharing m ths ->
-  ths[tid] --[EF_Alloc (length m) v V]--> t ->
+  ths[tid] --[EF_Alloc (#m) v V]--> t ->
   safe_memory_sharing (m +++ (v, V)) ths[tid <- t].
 Proof.
   intros * Hva ? ? tid1 tid2 ad Hneq Hacc1 Huacc.
   eapply uacc_then_acc in Huacc as Hacc2. contradict Huacc.
-  assert (tid < length ths) by eauto using length_tid.
+  assert (tid < #ths) by eauto using step_length_tid.
   destruct (Nat.eq_dec tid tid1), (Nat.eq_dec tid tid2); subst; try lia;
   simpl_array;
-  assert (ad <> length m)
+  assert (ad <> #m)
     by eauto 6 using mem_add_acc, mem_add_uacc, uacc_then_acc,
       vac_length, vac_nacc_length, Nat.lt_neq;
   eauto 6 using step_alloc_inherits_acc, step_alloc_nuacc_preservation,
@@ -89,7 +99,7 @@ Qed.
 
 Local Lemma step_read_sms_preservation : forall m t ad ths tid,
   forall_memory m value ->
-  forall_threads ths well_typed_thread ->
+  forall_threads ths well_typed ->
   forall_threads ths (well_typed_references m) ->
   safe_memory_sharing m ths ->
   ths[tid] --[EF_Read ad m[ad].tm]--> t ->
@@ -97,20 +107,20 @@ Local Lemma step_read_sms_preservation : forall m t ad ths tid,
 Proof.
   intros * ? Htype ? ? ? tid1 tid2 ? ? ?.
   destruct (Htype tid1).
-  assert (tid < length ths) by eauto using length_tid.
+  assert (tid < #ths) by eauto using step_length_tid.
   destruct (Nat.eq_dec tid tid1), (Nat.eq_dec tid tid2); subst; try lia;
   simpl_array; eauto using step_read_nuacc_preservation, step_read_inherits_acc.
 Qed.
 
 Local Lemma step_write_sms_preservation : forall m ths t tid ad v V,
-  forall_threads ths well_typed_thread ->
+  forall_threads ths well_typed ->
   safe_memory_sharing m ths ->
   ths[tid] --[EF_Write ad v V]--> t ->
   safe_memory_sharing m[ad <- (v, V)] ths[tid <- t].
 Proof.
   intros * ? ? ? tid1 tid2 ad' ? ? Huacc.
   eapply uacc_then_acc in Huacc as Hacc2. contradict Huacc.
-  assert (tid < length ths) by eauto using length_tid.
+  assert (tid < #ths) by eauto using step_length_tid.
   destruct (Nat.eq_dec tid tid1), (Nat.eq_dec tid tid2); subst; try lia;
   simpl_array;
   assert (~ UnsafeAccess m ths[tid1] ad');
@@ -122,7 +132,7 @@ Qed.
 Local Corollary mstep_sms_preservation : forall m m' t eff ths tid,
   forall_memory m value ->
   forall_threads ths (valid_accesses m) ->
-  forall_threads ths well_typed_thread ->
+  forall_threads ths well_typed ->
   forall_threads ths (well_typed_references m) ->
   safe_memory_sharing m ths ->
   m / ths[tid] ==[eff]==> m' / t ->
@@ -188,34 +198,61 @@ Proof.
 Qed.
 
 (* ------------------------------------------------------------------------- *)
-(* sms preservation                                                          *)
+(* preservation                                                              *)
 (* ------------------------------------------------------------------------- *)
 
 Theorem safe_memory_sharing_preservation : forall m m' ths ths' tid eff,
   forall_memory m value ->
-  forall_memory m (well_typed_references m) ->
-  forall_threads ths (valid_accesses m) ->
-  forall_threads ths well_typed_thread ->
-  forall_threads ths (well_typed_references m) ->
+  forall_threads ths well_typed ->
+  forall_program m ths (valid_addresses m) ->
+  forall_program m ths (well_typed_references m) ->
   forall_threads ths SafeSpawns ->
+  (* --- *)
   safe_memory_sharing m ths ->
-  tid < length ths ->
   m / ths ~~[tid, eff]~~> m' / ths' ->
   safe_memory_sharing m' ths'.
 Proof.
-  intros. inversion_clear_cstep; eauto using mstep_sms_preservation.
+  intros * ? ? [? ?] [? ?]. intros.
+  assert (tid < #ths) by eauto using cstep_length_tid.
+  assert (forall_threads ths (valid_accesses m))
+    by eauto using forall_threads_vad_then_vac.
+  inversion_clear_cstep; eauto using mstep_sms_preservation.
   assert (NoMut block) by eauto using nomut_block.
   intros tid1 tid2. intros.
   destruct (Nat.eq_dec tid tid1), (Nat.eq_dec tid tid2); subst; try lia;
-  decompose sum (lt_eq_lt_dec tid1 (length ths)); subst; simpl_array;
+  decompose sum (lt_eq_lt_dec tid1 (#ths)); subst; simpl_array;
   eauto using step_spawn_inherits_acc, step_spawn_nuacc_preservation;
   eauto using nomut_then_nuacc;
   eauto using nuacc_unit;
-  decompose sum (lt_eq_lt_dec tid2 (length ths)); subst; simpl_array;
+  decompose sum (lt_eq_lt_dec tid2 (#ths)); subst; simpl_array;
   eauto using step_spawn_inherits_acc, step_spawn_nuacc_preservation;
   unfold thread_default in *; try inversion_acc; intros ?;
   eauto using consistent_uacc,
     step_spawn_wtr_block, step_spawn_wtr_preservation,
     nomut_then_nuacc.
 Qed.
+
+From Elo Require Import Soundness.
+
+Theorem safe_memory_sharing_multistep_preservation :
+  forall m m' ths ths' tc,
+    forall_memory m value ->
+    forall_program m ths well_typed ->
+    forall_program m ths (valid_addresses m) ->
+    forall_program m ths (well_typed_references m) ->
+    forall_program m ths SafeSpawns ->
+    (* --- *)
+    safe_memory_sharing m ths ->
+    m / ths ~~[tc]~~>* m' / ths' ->
+    safe_memory_sharing m' ths'.
+Proof.
+  intros * ? ? ? ? ? ? Hmultistep. induction Hmultistep; trivial.
+  do 6 auto_specialize.
+  eapply (safe_memory_sharing_preservation m' m'' ths' ths''); eauto.
+  - admit.
+  - eapply well_typed_multistep_preservation; eauto.
+  - eapply valid_addresses_multistep_preservation; eauto.
+  - eapply well_typed_multistep_preservation; eauto.
+  - eapply safe_spawns_multistep_preservation; eauto.
+Abort.
 
