Safety.v
@@ -2,37 +2,43 @@ From Coq Require Import Arith.Arith.
 From Coq Require Import Lists.List.
 From Coq Require Import Lia.
 
+From Elo Require Import Util.
 From Elo Require Import Array.
-From Elo Require Import Core0.
+From Elo Require Import Map.
+From Elo Require Import Core.
 From Elo Require Import Access.
+From Elo Require Import UnsafeAccess.
+From Elo Require Import SMS.
 
 Reserved Notation "m / t '==[' tc ']==>*' m' / t'"
   (at level 40, t at next level, tc at next level,
                 m' at next level, t' at next level).
 
-Reserved Notation "m / t '~~[' tc ']~~>*' m' / t'"
-  (at level 40, t at next level, tc at next level,
-                m' at next level, t' at next level).
+Definition mtrace := list effect.
 
-Definition trace := list effect.
+(* ------------------------------------------------------------------------- *)
+(* reflexive transitive closure                                              *)
+(* ------------------------------------------------------------------------- *)
 
-(* reflexive transitive closure *)
-Inductive multistep : mem -> tm -> trace -> mem -> tm -> Prop :=
-  | multistep_refl: forall m t,
+Inductive mmultistep : mem -> tm -> mtrace -> mem -> tm -> Prop :=
+  | mmultistep_refl: forall m t,
     m / t ==[nil]==>* m / t
 
-  | multistep_trans : forall m m' m'' t t' t'' tc eff,
+  | mmultistep_trans : forall m m' m'' t t' t'' tc eff,
     m  / t  ==[tc]==>* m'  / t'  ->
     m' / t' ==[eff]==> m'' / t'' ->
     m  / t  ==[eff :: tc]==>* m'' / t''
 
-  where "m / t '==[' tc ']==>*' m' / t'" := (multistep m t tc m' t').
+  where "m / t '==[' tc ']==>*' m' / t'" := (mmultistep m t tc m' t').
 
-(* PART 1 *)
+
+(* ------------------------------------------------------------------------- *)
+(*                                                                           *)
+(* ------------------------------------------------------------------------- *)
 
 Lemma monotonic_nondecreasing_memory_length: forall m m' eff t t',
   m / t ==[eff]==>* m' / t' ->
-  length m <= length m'.
+  #m <= #m'.
 Proof.
   assert (forall m m' eff t t',
     m / t ==[eff]==> m' / t' ->
@@ -41,15 +47,14 @@ Proof.
     - rewrite add_increments_length. lia.
     - eauto using Nat.eq_le_incl, set_preserves_length.
   }
-  intros * Hmultistep. induction Hmultistep; eauto using Nat.le_trans.
+  intros * Hmmultistep. induction Hmmultistep; eauto using Nat.le_trans.
 Qed.
 
-Lemma alloc_increments_memory_length : forall m m' t t' ad v,
-  m / t ==[EF_Alloc ad v]==> m' / t' ->
-  length m' = S (length m).
+Lemma alloc_increments_memory_length : forall m m' t t' ad v Tr,
+  m / t ==[EF_Alloc ad v Tr]==> m' / t' ->
+  #m' = S (#m).
 Proof.
-  intros * Hmstep. inversion Hmstep; subst.
-  eauto using add_increments_length.
+  intros. inversion_mstep. eauto using add_increments_length.
 Qed.
 
 Lemma destruct_multistep : forall tc eff m0 mF t0 tF,
@@ -58,13 +63,13 @@ Lemma destruct_multistep : forall tc eff m0 mF t0 tF,
 Proof.
   intros ?. induction tc as [| eff tc IH];
   intros * Hmultistep; inversion Hmultistep; subst.
-  - eexists. eexists. inversion H3; subst. split; eauto using multistep.
+  - eexists. eexists. inversion H3; subst. split; eauto using mmultistep.
   - specialize (IH _ _ _ _ _ H3) as [? [? [? ?]]].
-    eexists. eexists. split; eauto using multistep.
+    eexists. eexists. split; eauto using mmultistep.
 Qed.
 
-Theorem duplicate_alloc : forall m m' t t' tc ad v v',
-  ~ (m / t ==[EF_Alloc ad v :: tc ++ EF_Alloc ad v' :: nil]==>* m' / t').
+Theorem duplicate_alloc : forall m m' t t' tc ad v v' Tr Tr',
+  ~ (m / t ==[EF_Alloc ad v Tr :: tc ++ EF_Alloc ad v' Tr' :: nil]==>* m' / t').
 Proof.
   assert (not_Sn_le_n : forall n, ~ (S n <= n)). {
     unfold not. intros * F. induction n;
@@ -102,87 +107,96 @@ Proof.
     lia.
 Qed.
 
-(* PART 4 *)
+(* ------------------------------------------------------------------------- *)
+(*                                                                           *)
+(* ------------------------------------------------------------------------- *)
 
-Local Lemma access_set : forall m t ad ad' v,
-  ~ access m t ad ->
-  ~ access m v ad ->
-  ~ access (set m ad' v) t ad.
+Local Lemma cstep_read_requires_acc : forall m m' ths ths' tid ad v,
+  m / ths ~~[tid, EF_Read ad v]~~> m' / ths' ->
+  access m ths[tid] ad.
 Proof.
-  assert (ge_iff_le : forall m n, m >= n <-> n <= m).
-  { intros. split; destruct n; eauto. }
-  assert (forall m ad ad' v,
-    access (set m ad' v) (get TM_Nil (set m ad' v) ad') ad ->
-    ad' < length m). {
-    intros * H. eapply not_ge. rewrite ge_iff_le. intros ?.
-    rewrite get_set_invalid in H; trivial. inversion H.
-  }
-  intros * HnaccT HnaccV F.
-  remember (set m ad' v) as m'.
-  induction F; inversion Heqm'; subst; eauto using access.
-  match goal with H : ~ access _ (TM_Loc ?ad) _ |- _ => 
-    destruct (Nat.eq_dec ad' ad) as [? | Hneq]; subst
-  end. 
-  - match goal with H : ~ access _ (TM_Loc ?ad) _ |- _ => 
-      assert (ad < length m); eauto
-    end. 
-    rewrite (get_set_eq TM_Nil) in F; trivial.
-    rewrite (get_set_eq TM_Nil) in IHF; eauto.
-  - eapply not_eq_sym in Hneq.
-    rewrite (get_set_neq TM_Nil) in *; eauto using access.
+  intros. inversion_clear_cstep. inversion_clear_mstep. induction_step;
+  eauto using access.
 Qed.
 
-Local Lemma access_add : forall m t ad v,
+Local Lemma cstep_write_requires_uacc : forall m m' ths ths' tid ad v Tr,
+  forall_threads ths well_typed ->
+  m / ths ~~[tid, EF_Write ad v Tr]~~> m' / ths' ->
+  UnsafeAccess m ths[tid] ad.
+Proof.
+  intros * Htype. intros. destruct (Htype tid) as [T ?].
+  inversion_clear_cstep. inversion_clear_mstep. generalize dependent T.
+  induction_step; intros; inversion_type; eauto using UnsafeAccess.
+  inversion_type. eauto using UnsafeAccess.
+Qed.
+
+Theorem safety : forall m m' ths ths' tid1 tid2 ad v v' tc Tr,
+  forall_threads ths well_typed ->
+  safe_memory_sharing m ths ->
+  tid1 <> tid2 ->
+  m / ths ~~[(tid1, EF_Read  ad v    ) :: tc ++
+             (tid2, EF_Write ad v' Tr) :: nil]~~>* m' / ths' ->
+  False.
+Proof.
+  intros * Htype Hsms Hneq Hcmultistep.
+  inversion_subst_clear Hcmultistep.
+  assert (Hacc : access m'0 ths'0[tid1] ad)
+    by eauto using cstep_read_requires_acc.
+  assert (safe_memory_sharing)
+  destruct tc.
+  - inversion H6; subst.
+    inversion H7; subst.
+    assert (Huacc : UnsafeAccess m'1 ths'1[tid2] ad)
+      by eauto using cstep_write_requires_uacc.
+
+Qed.
+
+
+(* ------------------------------------------------------------------------- *)
+(* TODO                                                                      *)
+(* ------------------------------------------------------------------------- *)
+
+Local Lemma access_add : forall m t ad v Tr,
   ~ access m t ad ->
   ~ access m v ad ->
-  ~ access (add m v) t ad.
+  ~ access (m +++ (v, Tr)) t ad.
 Proof.
   intros * HnaccT HnaccV Hacc.
   induction Hacc; eauto using access.
   eapply IHHacc; clear IHHacc; trivial.
-  decompose sum (lt_eq_lt_dec ad' (length m)); subst.
-  - rewrite (get_add_lt TM_Nil); eauto using access.
-  - rewrite (get_add_eq TM_Nil). trivial.
-  - rewrite (get_add_gt TM_Nil); trivial. intros ?. inversion_access.
+  decompose sum (lt_eq_lt_dec ad' (length m)); subst; simpl_array;
+  eauto using access. intros ?. unfold memory_default in *. simpl in *.
+  inversion_acc.
 Qed.
 
-Local Lemma not_access_stored_value : forall m t t' ad ad' v, 
+Local Lemma not_access_stored_value : forall m t t' ad ad' v Tr,
   ~ access m t ad ->
-  t --[ EF_Store ad' v ]--> t' ->
+  t --[EF_Write ad' v Tr]--> t' ->
   ~ access m v ad.
 Proof.
-  intros * Hnacc Hstep.
-  remember (EF_Store ad' v) as eff.
-  induction Hstep; inversion Heqeff; subst; eauto using access.
+  intros. induction_step; eauto using access.
 Qed.
 
-Local Lemma not_access_allocated_value : forall m t t' ad ad' v, 
+Local Lemma not_access_allocated_value : forall m t t' ad ad' v Tr,
   ~ access m t ad ->
-  t --[ EF_Alloc ad' v ]--> t' ->
+  t --[EF_Alloc ad' v Tr]--> t' ->
   ~ access m v ad.
 Proof.
-  intros * Hnacc Hstep.
-  remember (EF_Alloc ad' v) as eff.
-  induction Hstep; inversion Heqeff; subst; eauto using access.
+  intros * Hnacc Hstep. induction_step; eauto using access.
 Qed.
 
-Lemma access_granted_by_alloc_is_memory_length : forall m t t' ad v,
+Lemma access_granted_by_alloc_is_memory_length : forall m t t' ad v Tr,
   ~ access m t ad ->
-  t --[ EF_Alloc (length m) v ]--> t' ->
-  access (add m v) t' ad ->
+  t --[EF_Alloc (#m) v Tr]--> t' ->
+  access (m +++ (v, Tr)) t' ad ->
   ad = length m.
 Proof.
-  intros * Hnacc Hstep Hacc.
-  remember (EF_Alloc (length m) v) as eff.
-  induction Hstep; inversion Heqeff; subst; try (clear Heqeff);
-  eauto using access, load_access, load_access_inverse.
-  - eapply new_access_inverse in Hnacc.
-    inversion Hacc; clear Hacc; subst; trivial.
-    match goal with F : access _ _ _ |- _ => contradict F end.
-    rewrite get_add_eq. eapply access_add; eauto.
-  - eapply asg_access_inverse in Hnacc as [HnaccL ?].
-    match goal with IH : _ -> _ -> _ -> ?x |- ?x => eapply IH; eauto end.
-    eapply asg_access in Hacc as [? | ?]; eauto.
+  intros * Hnacc ? Hacc.
+  induction_step; inversion_nacc Hnacc; inversion_acc; eauto using access.
+  - match goal with F : access _ _ _ |- _ => contradict F end.
+    simpl_array. eapply access_add; eauto.
+  - do 2 auto_specialize. eapply IHstep.
+    eapply acc_asg in Hacc as [? | ?]; eauto.
     exfalso. eapply (not_access_allocated_value _ l) in HnaccL; eauto. 
     eapply (access_add _ r); eauto.
   - eapply asg_access_inverse in Hnacc as [? HnaccR].
@@ -210,36 +224,6 @@ Proof.
   - contradict Hacc. eauto using store_does_not_grant_access.
 Qed.
 
-Lemma access_dec : forall m t ad,
-  {access m t ad} + {~ access m t ad}.
-Proof.
-  intros. induction t.
-  - right. intros F. inversion F.
-  - right. intros F. inversion F.
-  - destruct (Nat.eq_dec n ad); subst; try solve [left; eauto using access].
-    (* decidable (access m (get TM_Nil m ad') ad) *)
-    admit.
-  - destruct IHt.
-    + left. eauto using access.
-    + right. eauto using access_new_inverse.
-  - destruct IHt.
-    + left. eauto using access.
-    + right. eauto using access_load_inverse.
-  - destruct IHt1, IHt2; try solve [left; eauto using access].
-    right. eauto using access_asg_inverse.
-  - destruct IHt1, IHt2; try solve [left; eauto using access].
-    right. eauto using access_seq_inverse.
-Abort.
-
-Lemma provar_para_tirar_o_axioma : forall m m' t t' eff ad v,
-  access m' t' ad ->
-  eff <> EF_Alloc ad v ->
-  m / t ==[eff]==> m' / t' ->
-  access m t ad.
-Proof.
-  intros * Hacc Hneq Hmstep.
-Abort.
-
 Theorem access_needs_alloc_multistep : forall m m' t t' ad tc,
   ~ access m t ad ->
   m / t ==[tc]==>* m' / t' ->
@@ -260,25 +244,6 @@ Qed.
 
 (* PART 6 *)
 
-Definition ctrace := list (nat * effect).
-
-Inductive cmultistep : mem -> threads -> ctrace -> mem -> threads -> Prop :=
-  | cmultistep_refl: forall m ths,
-    m / ths ~~[nil]~~>* m / ths
-
-  | cmultistep_trans : forall m m' m'' tid ths ths' ths'' tc eff,
-    m  / ths  ~~[tc]~~>* m'  / ths'  ->
-    m' / ths' ~~[tid, eff]~~> m'' / ths'' ->
-    m  / ths  ~~[(tid, eff) :: tc]~~>* m'' / ths''
-
-  where "m / t '~~[' tc ']~~>*' m' / t'" := (cmultistep m t tc m' t').
-
-Ltac destruct_cstep :=
-  match goal with
-    | [ H : _ / _ ~~[_, _]~~> _ / _ |- _ ] =>
-      inversion H; subst; clear H
-  end.
-
 Theorem concurrent_duplicate_alloc :
   forall m m' ths ths' tid tid' tc1 tc2 ad v v',
   ~ (m / ths ~~[tc1 ++ (tid , EF_Alloc ad v ) ::
@@ -286,58 +251,5 @@ Theorem concurrent_duplicate_alloc :
 Proof.
   intros * F. inversion F; subst; clear F.
 Abort.
-
-Theorem threads_dont_share_memory :
-  forall m m' ths ths' t1 t2 tid tid1 tid2 eff ad,
-  m' / ths' ~~[tid, eff]~~> m / ths ->
-  t1 = get TM_Nil ths tid1 ->
-  access m t1 ad ->
-  t2 = get TM_Nil ths tid2 ->
-  tid1 <> tid2 ->
-  ~ access m t2 ad.
-Proof.
-  intros * Hcstep Ht1 Hacc1 Hte Hneq.
-Abort.
-
-(*
-
-Teorema Final.
-
-m / ths ~~[tc]~~>* m' / ths'
-
-*)
-
-*)
-
-
-
-
-
-
-
-
-
-
-
-
-(* BAGUNÇA)
-
-Lemma inverse : forall m ad ad',
-  ad <> ad' ->
-  access m (TM_Loc ad') ad ->
-  access m (get TM_Nil m ad') ad.
-Proof.
-  intros * Hneq Hacc.
-  remember (TM_Loc ad') as t.
-  induction Hacc; inversion Heqt; subst; trivial.
-  lia.
-Qed.
-
-Inductive something :
-  | Something_Load
-    tid = alguma thread
-    m / ths ==> m' / ths' # Load tid 23
-    em todas as outras threads que não são tid,
-    não pode ter Loc 23
 
 *)
