Soundness.v
@@ -6,6 +6,7 @@ From Elo Require Import Util.
 From Elo Require Import Array.
 From Elo Require Import Map.
 From Elo Require Import Core.
+From Elo Require Import ValidAddresses.
 From Elo Require Import Access.
 From Elo Require Import References.
 
@@ -124,6 +125,24 @@ Proof.
   inversion_wtr; inversion_step; eauto.
   inversion_type; inversion_wtr; apply_deterministic_typing. eauto.
 Qed.
+
+
+
+
+
+
+
+
+Theorem well_typed_multistep_preservation : forall m m' ths ths' tc,
+  forall_program m ths (valid_addresses m) ->
+  (* --- *)
+  forall_program m ths well_typed ->
+  forall_program m ths (well_typed_references m) ->
+  m / ths ~~[tc]~~>* m' / ths' ->
+  forall_program m' ths' well_typed /\
+  forall_program m' ths' (well_typed_references m').
+Proof.
+Admitted.
 
 (*
 Ltac solve_with_steps :=
