Makefile
@@ -14,7 +14,6 @@ access: core
 	$(COQC) HasAddress.v
 	$(COQC) ValidAddresses.v
 	$(COQC) Access.v
-	$(COQC) ValidAccesses.v
 	$(COQC) Contains.v
 	$(COQC) References.v
 
@@ -22,10 +21,10 @@ soundness: access
 	$(COQC) Soundness.v
 
 safety: soundness 
-	$(COQC) AccessProp.v
 	$(COQC) UnsafeAccess.v
 	$(COQC) SafeSpawns.v
 	$(COQC) SMS.v
+	$(COQC) Safety.v
 
 clean:
 	rm -f .lia.cache .*.aux *.vo *.vok *.vos *.glob
